Finished definition of rho and proof of invariance by renaming

pcuic/theories/PCUICDepth.v
@@ -58,7 +58,7 @@ Fixpoint depth t : nat :=
 Notation context_depth := (context_depth_gen depth).
 Notation list_depth := (list_depth_gen depth).
 
-  Lemma depth_mkApps f l : max (depth f) (list_depth l) <= depth (mkApps f l).
+Lemma depth_mkApps f l : max (depth f) (list_depth l) <= depth (mkApps f l).
 Proof.
   induction l in f |- *; simpl; try lia.
   specialize (IHl (tApp f a)).
@@ -288,7 +288,9 @@ Lemma term_forall_ctx_list_ind :
     (forall Γ (n : aname) (t : term), P Γ t -> forall t0 : term, P (vass n t :: Γ) t0 -> P Γ (tLambda n t t0)) ->
     (forall Γ (n : aname) (t : term),
         P Γ t -> forall t0 : term, P Γ t0 -> forall t1 : term, P (vdef n t t0 :: Γ) t1 -> P Γ (tLetIn n t t0 t1)) ->
-    (forall Γ (t u : term), P Γ t -> P Γ u -> P Γ (tApp t u)) ->
+    (forall Γ (t u : term), 
+      (forall t', depth t' < depth (tApp t u) -> P Γ t') ->
+      P Γ t -> P Γ u -> P Γ (tApp t u)) ->
     (forall Γ s (u : list Level.t), P Γ (tConst s u)) ->
     (forall Γ (i : inductive) (u : list Level.t), P Γ (tInd i u)) ->
     (forall Γ (i : inductive) (n : nat) (u : list Level.t), P Γ (tConstruct i n u)) ->
@@ -379,7 +381,127 @@ Proof.
         lia.
         eapply auxbr. unfold branch_depth_gen. lia.
       + eapply IHbrs. intros. apply auxΓ. simpl in *. lia.
-        intros. apply auxbr. simpl. lia.        
+        intros. apply auxbr. simpl. lia.
+  - eapply X12; try (apply aux; red; simpl; lia).
+    apply auxΓ => //. simpl. specialize (H mfix). lia.
+    red. apply All_pair. split; apply auxl; simpl; auto.
+
+  - eapply X13; try (apply aux; red; simpl; lia).
+    apply auxΓ => //. simpl. specialize (H mfix). lia.
+    red. apply All_pair. split; apply auxl; simpl; auto.
+Defined.
+
+Definition CasePredProp_depth (P : term -> Type) (p : predicate term) :=
+  All P p.(pparams) × onctx P (inst_case_context p.(pparams) p.(puinst) p.(pcontext)) ×
+  P p.(preturn).
+
+Definition CaseBrsProp_depth p (P : term -> Type) (brs : list (branch term)) :=
+  All (fun x : branch term => onctx P (inst_case_context p.(pparams) p.(puinst) x.(bcontext))
+     * P (bbody x)) brs.
+
+Lemma term_ind_depth_app :
+  forall (P : term -> Type),
+    (forall (n : nat), P (tRel n)) ->
+    (forall (i : ident), P (tVar i)) ->
+    (forall (n : nat) (l : list term), All (P) l -> P (tEvar n l)) ->
+    (forall s, P (tSort s)) ->
+    (forall (n : aname) (t : term), P t -> forall t0 : term, P t0 -> P (tProd n t t0)) ->
+    (forall (n : aname) (t : term), P t -> forall t0 : term, P t0 -> P (tLambda n t t0)) ->
+    (forall (n : aname) (t : term),
+        P t -> forall t0 : term, P t0 -> forall t1 : term, P t1 -> P (tLetIn n t t0 t1)) ->
+    (forall (t u : term), 
+      (forall t', depth t' < depth (tApp t u) -> P t') ->
+      P t -> P u -> P (tApp t u)) ->
+    (forall s (u : list Level.t), P (tConst s u)) ->
+    (forall (i : inductive) (u : list Level.t), P (tInd i u)) ->
+    (forall (i : inductive) (n : nat) (u : list Level.t), P (tConstruct i n u)) ->
+    (forall (ci : case_info) (p : predicate term) (t : term) (brs : list (branch term)),
+        CasePredProp_depth P p -> 
+        P t ->
+        CaseBrsProp_depth p P brs ->
+        P (tCase ci p t brs)) ->
+    (forall (s : projection) (t : term), P t -> P (tProj s t)) ->
+    (forall (m : mfixpoint term) (n : nat),
+        onctx P (fix_context m) ->
+        tFixProp P P m -> P (tFix m n)) ->
+    (forall (m : mfixpoint term) (n : nat),
+        onctx P (fix_context m) ->
+        tFixProp P P m -> P (tCoFix m n)) ->
+    (forall p, P (tPrim p)) ->
+    forall (t : term), P t.
+Proof.
+  intros ????????????????? t.
+  revert t. set(foo:=CoreTactics.the_end_of_the_section). intros.
+  Subterm.rec_wf_rel aux t (MR lt depth); unfold MR in *; simpl. clear H0.
+  assert (auxl : forall {A} (l : list A) (f : A -> term),
+    list_depth_gen (fun x => depth (f x)) l < depth pr1 ->
+    All (fun x => P (f x)) l).
+  { induction l; try solve [constructor].
+    move=> f /= Hdepth.
+    constructor.
+    * eapply aux => //. red. lia.
+    * apply IHl => //. lia. }
+  assert (forall mfix, context_depth (fix_context mfix) <= mfixpoint_depth_gen depth mfix).
+  { induction mfix. simpl. auto. simpl. unfold fix_context.
+    unfold context_depth.
+    rewrite /context_depth list_depth_rev /=. cbn.
+    rewrite depth_lift. unfold context_depth in IHmfix.
+    epose (list_depth_mapi_rec_le mfix
+                                 (fun (i : nat) (d : def term) => vass (dname d) ((lift0 i) (dtype d))) 1
+                                 (def_depth_gen depth) (decl_depth_gen depth)).
+    forward l. intros. destruct x; cbn; rewrite depth_lift. lia.
+    rewrite /mfixpoint_depth_gen {1}/def_depth_gen. lia. }
+  assert (auxΓ : forall Δ,
+             context_depth Δ < depth pr1 ->
+             onctx P Δ).
+  { move=> Γ h.
+    induction Γ; cbn.
+    - constructor.
+    - case: a h => [na [b|] ty] /=;
+      rewrite {1}/decl_depth_gen /context_depth_gen /= => Hlt; constructor; auto.
+      + simpl. split.
+        * apply aux => //. red. cbn. lia.
+        * apply aux=> //; red; lia.
+      + apply IHΓ => //; unfold context_depth; lia.
+      + red; cbn. split. apply aux => //. red. lia. exact tt.
+      + apply IHΓ => //. unfold context_depth; lia. }
+  assert (forall m, list_depth_gen (fun x : def term => depth (dtype x)) m < S (mfixpoint_depth_gen depth m)).
+  { clear. unfold mfixpoint_depth_gen, def_depth_gen. induction m. simpl. auto. simpl. lia. }
+  assert (forall m, list_depth_gen (fun x : def term => depth (dbody x)) m < S (mfixpoint_depth_gen depth m)).
+  { clear. unfold mfixpoint_depth_gen, def_depth_gen. induction m. simpl. auto. simpl. lia. }
+
+  move aux at top. move auxl at top. move auxΓ at top.
+
+  destruct pr1; eauto;
+    (move: pr2=> /= /and3P [pr20 pr21 pr22] || move: pr2 => /= /andP [pr20 pr21] || idtac);
+    try match reverse goal with
+          |- context [tFix _ _] => idtac
+        | H : _ |- _ => solve [apply H; (eapply aux || eapply auxl); auto; red; simpl; try lia]
+        end.
+
+  - eapply X10; eauto.
+    * red. split.
+      + eapply auxl; auto. simpl. unfold predicate_depth_gen, branch_depth_gen.
+        now change (fun x => depth x) with depth; lia.
+      + split.
+        ++ apply auxΓ. simpl. unfold predicate_depth_gen.
+          pose proof (context_depth_inst_case_context p.(pparams) p.(puinst) p.(pcontext)). lia.
+        ++ eapply aux; auto. simpl. unfold predicate_depth_gen. lia.
+    * eapply aux => //. simpl; lia.
+    * red. simpl in aux.
+      have auxbr := fun t (H : depth t <= list_depth_gen (branch_depth_gen depth p) brs) => 
+        aux t ltac:(lia).
+      move: auxbr.
+      clear -auxΓ.
+      induction brs. simpl. constructor.
+      constructor. simpl in auxbr.
+      + split. eapply auxΓ. simpl.
+        unfold branch_depth_gen at 1. rewrite /predicate_depth_gen /=.
+        pose proof (context_depth_inst_case_context p.(pparams) p.(puinst) a.(bcontext)).
+        lia.
+        eapply auxbr. unfold branch_depth_gen. lia.
+      + eapply IHbrs. intros. apply auxΓ. simpl in *. lia.
+        intros. apply auxbr. simpl. lia.
   - eapply X12; try (apply aux; red; simpl; lia).
     apply auxΓ => //. simpl. specialize (H mfix). lia.
     red. apply All_pair. split; apply auxl; simpl; auto.
